theory/Static_Communication_Analysis_Soundness.thy
@@ -76,7 +76,7 @@ lemma isnt_send_path_sound': "
     \<rho>\<^sub>e x\<^sub>s\<^sub>c = Some \<lbrace>Ch \<pi> x\<^sub>c\<rbrace>;
     \<E>' (\<pi>\<^sub>y;;`x\<^sub>y) = Some (\<langle>e\<^sub>y;\<rho>\<^sub>y(x\<^sub>y \<mapsto> \<lbrace>\<rbrace>);\<kappa>\<^sub>y\<rangle>) 
   \<rbrakk> \<Longrightarrow> 
-  \<V> \<turnstile> e \<down> (\<pi>\<^sub>y, LET x\<^sub>y = SYNC x\<^sub>e in e\<^sub>y) \<and>
+  \<V> \<turnstile> e \<down> \<pi>\<^sub>y \<mapsto> LET x\<^sub>y = SYNC x\<^sub>e in e\<^sub>y \<and>
   ^Chan x\<^sub>c \<in> \<V> x\<^sub>s\<^sub>c \<and>
   {^Send_Evt x\<^sub>s\<^sub>c x\<^sub>m} \<subseteq> \<V> x\<^sub>e
 
@@ -310,7 +310,7 @@ lemma isnt_recv_path_sound': "
     \<rho>\<^sub>e x\<^sub>r\<^sub>c = Some \<lbrace>Ch \<pi> x\<^sub>c\<rbrace>;
     \<E>' (\<pi>\<^sub>y;;`x\<^sub>y) = Some (\<langle>e\<^sub>y;\<rho>\<^sub>y(x\<^sub>y \<mapsto> \<omega>);\<kappa>\<^sub>y\<rangle>) 
   \<rbrakk> \<Longrightarrow>
-  \<V> \<turnstile> e \<down> (\<pi>\<^sub>y, LET x\<^sub>y = SYNC x\<^sub>e in e\<^sub>y) \<and>
+  \<V> \<turnstile> e \<down> \<pi>\<^sub>y \<mapsto> LET x\<^sub>y = SYNC x\<^sub>e in e\<^sub>y \<and>
   ^Chan x\<^sub>c \<in> \<V> x\<^sub>r\<^sub>c \<and>
   {^Recv_Evt x\<^sub>r\<^sub>c} \<subseteq> \<V> x\<^sub>e
 "
